isabelle/CVM_Original/CVM_Algo.thy
@@ -43,10 +43,7 @@ definition step_2 :: \<open>'a state \<Rightarrow> 'a state pmf\<close> where
     in if card chi = threshold
       then do {
         keep_in_chi :: 'a \<Rightarrow> bool \<leftarrow> prod_pmf chi \<lblot>bernoulli_pmf f\<rblot>;
-
-        let chi = Set.filter keep_in_chi chi;
-
-        return_pmf (\<lparr>state_k = k + 1, state_chi = chi\<rparr>) }
+        return_pmf (\<lparr>state_k = k + 1, state_chi = Set.filter keep_in_chi chi\<rparr>) }
       else return_pmf state\<close>
 
 definition step_3 :: \<open>'a state \<Rightarrow> 'a state spmf\<close> where
